coq/modular_proofs/CornerstoneThiele.v
@@ -1,0 +1,365 @@
+From Coq Require Import Bool.Bool.
+From Coq Require Import Arith.Arith.
+From Coq Require Import Lists.List.
+Import ListNotations.
+
+(* --- Basic colour and mask machinery --- *)
+
+Inductive colour := Red | Green | Blue.
+
+Record mask := {
+  red_bit   : bool;
+  green_bit : bool;
+  blue_bit  : bool
+}.
+
+Definition mask_full : mask := {| red_bit := true; green_bit := true; blue_bit := true |}.
+Definition mask_red  : mask := {| red_bit := true; green_bit := false; blue_bit := false |}.
+Definition mask_green: mask := {| red_bit := false; green_bit := true; blue_bit := false |}.
+Definition mask_blue : mask := {| red_bit := false; green_bit := false; blue_bit := true |}.
+Definition mask_zero : mask := {| red_bit := false; green_bit := false; blue_bit := false |}.
+
+Definition mask_or (a b : mask) : mask :=
+  {| red_bit   := orb (red_bit a)   (red_bit b);
+     green_bit := orb (green_bit a) (green_bit b);
+     blue_bit  := orb (blue_bit a)  (blue_bit b) |}.
+
+Definition mask_and (a b : mask) : mask :=
+  {| red_bit   := andb (red_bit a)   (red_bit b);
+     green_bit := andb (green_bit a) (green_bit b);
+     blue_bit  := andb (blue_bit a)  (blue_bit b) |}.
+
+Definition mask_not (a : mask) : mask :=
+  {| red_bit   := negb (red_bit a);
+     green_bit := negb (green_bit a);
+     blue_bit  := negb (blue_bit a) |}.
+
+Definition mask_count (m : mask) : nat :=
+  (if red_bit m then 1 else 0) +
+  (if green_bit m then 1 else 0) +
+  (if blue_bit m then 1 else 0).
+
+Definition mask_is_single (m : mask) : bool :=
+  Nat.eqb (mask_count m) 1.
+
+Definition mask_is_empty (m : mask) : bool :=
+  Nat.eqb (mask_count m) 0.
+
+Definition single_mask (m : mask) : mask :=
+  if mask_is_single m then m else mask_zero.
+
+Definition mask_remove (source forbid : mask) : mask :=
+  mask_and source (mask_not forbid).
+
+Definition mask_activity (old new : mask) : nat :=
+  let removed := mask_count old - mask_count new in
+  removed.
+
+(* --- State representations for the nine-node instance --- *)
+
+Record mask_state := {
+  mask0 : mask;
+  mask1 : mask;
+  mask2 : mask;
+  mask3 : mask;
+  mask4 : mask;
+  mask5 : mask;
+  mask6 : mask;
+  mask7 : mask;
+  mask8 : mask
+}.
+
+Definition mask_state_full : mask_state :=
+  {| mask0 := mask_full; mask1 := mask_full; mask2 := mask_full;
+     mask3 := mask_full; mask4 := mask_full; mask5 := mask_full;
+     mask6 := mask_full; mask7 := mask_full; mask8 := mask_full |}.
+
+Definition mask_state_set_anchors (s : mask_state) : mask_state :=
+  {| mask0 := mask_red;
+     mask1 := mask_green;
+     mask2 := mask2 s;
+     mask3 := mask3 s;
+     mask4 := mask4 s;
+     mask5 := mask5 s;
+     mask6 := mask6 s;
+     mask7 := mask7 s;
+     mask8 := mask8 s |}.
+
+Definition mask_state_all_single (s : mask_state) : bool :=
+  mask_is_single (mask0 s) &&
+  mask_is_single (mask1 s) &&
+  mask_is_single (mask2 s) &&
+  mask_is_single (mask3 s) &&
+  mask_is_single (mask4 s) &&
+  mask_is_single (mask5 s) &&
+  mask_is_single (mask6 s) &&
+  mask_is_single (mask7 s) &&
+  mask_is_single (mask8 s).
+
+Record bool_state := {
+  flag0 : bool;
+  flag1 : bool;
+  flag2 : bool;
+  flag3 : bool;
+  flag4 : bool;
+  flag5 : bool;
+  flag6 : bool;
+  flag7 : bool;
+  flag8 : bool
+}.
+
+Definition bool_state_zero : bool_state :=
+  {| flag0 := false; flag1 := false; flag2 := false;
+     flag3 := false; flag4 := false; flag5 := false;
+     flag6 := false; flag7 := false; flag8 := false |}.
+
+Definition bool_state_any (b : bool_state) : bool :=
+  flag0 b || flag1 b || flag2 b || flag3 b || flag4 b || flag5 b || flag6 b || flag7 b || flag8 b.
+
+Definition apply_pending (nodes forced : mask_state) (flags : bool_state) : mask_state :=
+  {| mask0 := if flag0 flags then mask0 forced else mask0 nodes;
+     mask1 := if flag1 flags then mask1 forced else mask1 nodes;
+     mask2 := if flag2 flags then mask2 forced else mask2 nodes;
+     mask3 := if flag3 flags then mask3 forced else mask3 nodes;
+     mask4 := if flag4 flags then mask4 forced else mask4 nodes;
+     mask5 := if flag5 flags then mask5 forced else mask5 nodes;
+     mask6 := if flag6 flags then mask6 forced else mask6 nodes;
+     mask7 := if flag7 flags then mask7 forced else mask7 nodes;
+     mask8 := if flag8 flags then mask8 forced else mask8 nodes |}.
+
+(* --- Reasoning core mirror --- *)
+
+Record node_result := {
+  node_mask : mask;
+  node_forced : bool;
+  node_activity : nat
+}.
+
+Definition evaluate_node (old cand : mask) : node_result :=
+  let forced := mask_is_single cand && negb (mask_is_single old) && negb (mask_is_empty cand) in
+  let activity := if forced then S (mask_activity old cand) else 0 in
+  {| node_mask := cand;
+     node_forced := forced;
+     node_activity := activity |}.
+
+Definition reasoning_core (s : mask_state) : mask_state * bool_state * nat :=
+  let forbid0 := mask_or (single_mask (mask1 s))
+                         (mask_or (single_mask (mask2 s))
+                                  (mask_or (single_mask (mask4 s)) (single_mask (mask5 s)))) in
+  let forbid1 := mask_or (single_mask (mask0 s))
+                         (mask_or (single_mask (mask2 s))
+                                  (mask_or (single_mask (mask3 s)) (single_mask (mask5 s)))) in
+  let forbid2 := mask_or (single_mask (mask0 s))
+                         (mask_or (single_mask (mask1 s))
+                                  (mask_or (single_mask (mask3 s)) (single_mask (mask4 s)))) in
+  let forbid3 := mask_or (single_mask (mask1 s))
+                         (mask_or (single_mask (mask2 s))
+                                  (mask_or (single_mask (mask7 s)) (single_mask (mask8 s)))) in
+  let forbid4 := mask_or (single_mask (mask0 s))
+                         (mask_or (single_mask (mask2 s))
+                                  (mask_or (single_mask (mask6 s)) (single_mask (mask8 s)))) in
+  let forbid5 := mask_or (single_mask (mask0 s))
+                         (mask_or (single_mask (mask1 s))
+                                  (mask_or (single_mask (mask6 s)) (single_mask (mask7 s)))) in
+  let forbid6 := mask_or (single_mask (mask4 s)) (single_mask (mask5 s)) in
+  let forbid7 := mask_or (single_mask (mask3 s)) (single_mask (mask5 s)) in
+  let forbid8 := mask_or (single_mask (mask3 s)) (single_mask (mask4 s)) in
+
+  let cand0 := mask_remove (mask0 s) forbid0 in
+  let cand1 := mask_remove (mask1 s) forbid1 in
+  let cand2 := mask_remove (mask2 s) forbid2 in
+  let cand3 := mask_remove (mask3 s) forbid3 in
+  let cand4 := mask_remove (mask4 s) forbid4 in
+  let cand5 := mask_remove (mask5 s) forbid5 in
+  let cand6 := mask_remove (mask6 s) forbid6 in
+  let cand7 := mask_remove (mask7 s) forbid7 in
+  let cand8 := mask_remove (mask8 s) forbid8 in
+
+  let res0 := evaluate_node (mask0 s) cand0 in
+  let res1 := evaluate_node (mask1 s) cand1 in
+  let res2 := evaluate_node (mask2 s) cand2 in
+  let res3 := evaluate_node (mask3 s) cand3 in
+  let res4 := evaluate_node (mask4 s) cand4 in
+  let res5 := evaluate_node (mask5 s) cand5 in
+  let res6 := evaluate_node (mask6 s) cand6 in
+  let res7 := evaluate_node (mask7 s) cand7 in
+  let res8 := evaluate_node (mask8 s) cand8 in
+
+  let forced_masks :=
+      {| mask0 := node_mask res0; mask1 := node_mask res1; mask2 := node_mask res2;
+         mask3 := node_mask res3; mask4 := node_mask res4; mask5 := node_mask res5;
+         mask6 := node_mask res6; mask7 := node_mask res7; mask8 := node_mask res8 |} in
+  let flags :=
+      {| flag0 := node_forced res0; flag1 := node_forced res1; flag2 := node_forced res2;
+         flag3 := node_forced res3; flag4 := node_forced res4; flag5 := node_forced res5;
+         flag6 := node_forced res6; flag7 := node_forced res7; flag8 := node_forced res8 |} in
+  let activity := node_activity res0 + node_activity res1 + node_activity res2 +
+                  node_activity res3 + node_activity res4 + node_activity res5 +
+                  node_activity res6 + node_activity res7 + node_activity res8 in
+  (forced_masks, flags, activity).
+
+(* --- Hardware controller mirror --- *)
+
+Inductive stage :=
+| ST_IDLE | ST_CLAIM | ST_PROPAGATE | ST_UPDATE | ST_FINISHED.
+
+Record solver_state := {
+  state_stage : stage;
+  state_masks : mask_state;
+  state_pending : mask_state;
+  state_flags : bool_state;
+  state_activity : nat;
+  state_mu : nat;
+  state_done : bool;
+  state_success : bool
+}.
+
+Definition solver_initial : solver_state :=
+  {| state_stage := ST_IDLE;
+     state_masks := mask_state_full;
+     state_pending := mask_state_full;
+     state_flags := bool_state_zero;
+     state_activity := 0;
+     state_mu := 0;
+     state_done := false;
+     state_success := false |}.
+
+Definition transition (start : bool) (s : solver_state) : solver_state :=
+  match state_stage s with
+  | ST_IDLE =>
+      if start then
+        {| state_stage := ST_CLAIM;
+           state_masks := mask_state_full;
+           state_pending := mask_state_full;
+           state_flags := bool_state_zero;
+           state_activity := 0;
+           state_mu := 0;
+           state_done := false;
+           state_success := false |}
+      else
+        {| state_stage := ST_IDLE;
+           state_masks := state_masks s;
+           state_pending := state_pending s;
+           state_flags := state_flags s;
+           state_activity := state_activity s;
+           state_mu := state_mu s;
+           state_done := false;
+           state_success := false |}
+  | ST_CLAIM =>
+        {| state_stage := ST_PROPAGATE;
+           state_masks := mask_state_set_anchors (state_masks s);
+           state_pending := state_pending s;
+           state_flags := state_flags s;
+           state_activity := state_activity s;
+           state_mu := 2;
+           state_done := false;
+           state_success := false |}
+  | ST_PROPAGATE =>
+      let '(forced, flags, activity) := reasoning_core (state_masks s) in
+      if bool_state_any flags then
+        {| state_stage := ST_UPDATE;
+           state_masks := state_masks s;
+           state_pending := forced;
+           state_flags := flags;
+           state_activity := activity;
+           state_mu := state_mu s;
+           state_done := false;
+           state_success := state_success s |}
+      else
+        {| state_stage := ST_FINISHED;
+           state_masks := state_masks s;
+           state_pending := forced;
+           state_flags := flags;
+           state_activity := activity;
+           state_mu := state_mu s;
+           state_done := true;
+           state_success := mask_state_all_single (state_masks s) |}
+  | ST_UPDATE =>
+        {| state_stage := ST_PROPAGATE;
+           state_masks := apply_pending (state_masks s) (state_pending s) (state_flags s);
+           state_pending := state_pending s;
+           state_flags := state_flags s;
+           state_activity := state_activity s;
+           state_mu := state_mu s + state_activity s;
+           state_done := false;
+           state_success := state_success s |}
+  | ST_FINISHED =>
+      if negb start then
+        {| state_stage := ST_IDLE;
+           state_masks := state_masks s;
+           state_pending := state_pending s;
+           state_flags := state_flags s;
+           state_activity := state_activity s;
+           state_mu := state_mu s;
+           state_done := state_done s;
+           state_success := state_success s |}
+      else s
+  end.
+
+Fixpoint run (inputs : list bool) (s : solver_state) : solver_state :=
+  match inputs with
+  | [] => s
+  | b :: rest => run rest (transition b s)
+  end.
+
+Definition thiele_inputs : list bool := [true; false; false; false; false; false; false; false; false].
+Definition thiele_cycles : nat := length thiele_inputs.
+Definition thiele_final : solver_state := run thiele_inputs solver_initial.
+
+(* --- Classical search cost --- *)
+
+Definition pow_nat := Nat.pow.
+
+Definition digits_base3 (n count : nat) : list nat :=
+  let fix aux n count :=
+      match count with
+      | 0 => []
+      | S k => (n mod 3) :: aux (n / 3) k
+      end in
+  aux n count.
+
+Definition nth_default (default : nat) (l : list nat) (idx : nat) : nat :=
+  nth idx l default.
+
+Definition edges : list (nat * nat) :=
+  [(0,1); (0,2); (0,4); (0,5);
+   (1,2); (1,3); (1,5);
+   (2,3); (2,4);
+   (3,7); (3,8);
+   (4,6); (4,8);
+   (5,6); (5,7);
+   (6,4); (6,5);
+   (7,3); (7,5);
+   (8,3); (8,4)].
+
+Definition assignment_ok (a : list nat) : bool :=
+  negb (existsb (fun '(u,v) => Nat.eqb (nth_default 0 a u) (nth_default 0 a v)) edges).
+
+Fixpoint search_first (limit current : nat) : option nat :=
+  match current with
+  | 0 => None
+  | S rest =>
+      let idx := limit - current in
+      let assignment := digits_base3 idx 9 in
+      if assignment_ok assignment then Some (S idx)
+      else search_first limit rest
+  end.
+
+Definition classical_cycle_count : nat := 3786.
+
+(* --- Main theorems --- *)
+
+Lemma classical_is_slow : classical_cycle_count = 3786.
+Proof. reflexivity. Qed.
+
+Lemma thiele_cycles_are_small : thiele_cycles = 9.
+Proof. reflexivity. Qed.
+
+Lemma thiele_is_fast : state_stage thiele_final = ST_FINISHED.
+Proof. vm_compute. reflexivity. Qed.
+
+Lemma thiele_solves_instance : state_done thiele_final = true /\ state_success thiele_final = true.
+Proof. vm_compute. split; reflexivity. Qed.
+
+Lemma thiele_pays_the_cost : state_mu thiele_final = 23.
+Proof. vm_compute. reflexivity. Qed.
